\documentclass[]{article}
\usepackage{amsmath}
\begin{document}

\title{Title}
\author{Author}
\date{Today}
\maketitle

 $$\frac{dz}{dt} = z\left(\alpha + \textrm{i}\omega + 
 \beta_1 |z|^2 + \frac{\epsilon\beta_2|z|^4}
 {1-\epsilon |z|^2}\right) + Fe^{\textrm{i}\theta}$$

 where $z = re^{\textrm{i}\phi}, \psi = \phi - \theta,
 \theta = \omega_0t + \theta_0, ~and~ \Omega = \omega - \omega_0$\\\\

\noindent 
To find the steady-state amplitude we solve $\dot{r} = 0$

\begin{align*}
\dot{r} &= \alpha r + \beta_1r^3 +\frac{\epsilon \beta_2 r^5 }{1 - \epsilon r^2}\\
0 &= \alpha r + \beta_1r^3 +\frac{\epsilon \beta_2 r^5 }{1 - \epsilon r^2}\\
-\frac{\epsilon \beta_2 r^5 }{1 - \epsilon r^2} &= \alpha r + \beta_1r^3 \\
-\epsilon \beta_2 r^5  &= (\alpha r + \beta_1r^3)(1 - \epsilon r^2) \\
&= \alpha r + \beta_1r^3 - \epsilon \alpha r^3 - \epsilon \beta_1 r^5 \\
0 &= \alpha r + \beta_1r^3 - \epsilon \alpha r^3 - \epsilon \beta_1 r^5 + \epsilon \beta_2 r^5\\
&= \alpha r + (\beta_1 - \epsilon \alpha) r^3 - \epsilon (\beta_2 - \beta_1) r^5\\
\end{align*}

\end{document}